Move several files around, depend on coqrel

src/FunMaps.v
@@ -7,28 +7,107 @@ Require Import
   Coq.Structures.OrderedTypeEx.
 
 Require Import
-  Here.LogicalRelations
+  CoqRel.LogicalRelations
   Coq.Classes.Morphisms
   Coq.Classes.RelationClasses
   Coq.Setoids.Setoid
   Coq.Classes.Equivalence
   Here.Same_set.
 
+Notation "f [R  rel ] f'" := (Related rel f f')
+  (right associativity, at level 55) : rel_scope.
+
 Module FunMaps (O : OrderedType).
 
 Module E := FMapExt(O).
 Include E.
 
-Definition Map_AbsR (A B : Type) (R : A -> B -> Prop)
-           (or : Ensemble (M.key * A)) (nr : M.t B) : Prop :=
-  forall addr,
-    (forall blk,
-       Lookup addr blk or
-         -> (exists cblk, M.find addr nr = Some cblk /\ R blk cblk)) /\
-    (forall cblk,
-       M.find addr nr = Some cblk
-         -> (exists blk, Lookup addr blk or /\ R blk cblk)).
+Open Scope rel_scope.
 
+Class DeterminingRelation {A B : Type} (R : A -> B -> Prop) := {
+  R_injective  : forall a, exists b, R a b;
+  R_surjective : forall b, exists a, R a b;
+  A_determines_B : forall a b b', R a b -> R a b' -> b = b';
+  B_determines_A : forall a a' b, R a b -> R a' b -> a = a'
+}.
+
+Arguments A_determines_B {A B} R {_ a b b'} _ _.
+Arguments B_determines_A {A B} R {_ a a' b} _ _.
+
+Definition Map_AbsR {A B : Type} (R : A -> B -> Prop)
+           (or : Ensemble (M.key * A)) (nr : M.t B) : Prop :=
+  forall addr blk cblk `{DeterminingRelation A B R},
+    R blk cblk -> (Lookup addr blk or <-> M.find addr nr = Some cblk).
+
+Ltac reduction :=
+  try repeat teardown; subst;
+  repeat match goal with
+  | [ R : ?A -> ?B -> Prop,
+      H : DeterminingRelation ?R,
+      H1 : Map_AbsR ?R ?X ?Y,
+      H2 : Lookup ?ADDR ?BLK ?X,
+      H3 : ?R ?BLK ?CBLK |- _ ] =>
+    apply (H1 ADDR BLK CBLK H H3) in H2; clear H1
+  | [ R : ?A -> ?B -> Prop,
+      H : DeterminingRelation ?R,
+      H1 : Map_AbsR ?R ?X ?Y,
+      H2 : Lookup ?ADDR ?BLK ?X |- _ ] =>
+    let cblk := fresh "cblk" in
+    destruct (R_injective BLK) as [cblk ?]
+  | [ H1 : Map_AbsR ?R ?X ?Y,
+      H2 : Lookup ?ADDR ?BLK ?Z,
+      H3 : Same ?X ?Z |- _ ] =>
+    apply H3 in H2
+  | [ H1 : Map_AbsR ?R ?X ?Y,
+      H2 : Lookup ?ADDR ?BLK ?Z,
+      H3 : Same ?Z ?X |- _ ] =>
+    apply H3 in H2
+  | [ R : ?A -> ?B -> Prop,
+      H : DeterminingRelation ?R,
+      H1 : Map_AbsR ?R ?X ?Y,
+      H2 : M.find ?ADDR ?Y = Some ?CBLK,
+      H3 : ?R ?BLK ?CBLK |- _ ] =>
+    apply (H1 ADDR BLK CBLK H H3) in H2; clear H1
+  | [ R : ?A -> ?B -> Prop,
+      H : DeterminingRelation ?R,
+      H1 : Map_AbsR ?R ?X ?Y,
+      H2 : M.find ?ADDR ?Y = Some ?CBLK |- _ ] =>
+    let cblk := fresh "cblk" in
+    destruct (R_surjective CBLK) as [blk ?]
+  | [ H1 : Map_AbsR ?R ?X ?Y,
+      H2 : M.find ?ADDR ?Z = Some ?CBLK,
+      H3 : M.Equal ?Y ?Z |- _ ] =>
+    rewrite <- H3 in H2
+  | [ H1 : Map_AbsR ?R ?X ?Y,
+      H2 : M.find ?ADDR ?Z = Some ?CBLK,
+      H3 : M.Equal ?Z ?Y |- _ ] =>
+    rewrite H3 in H2
+  | [ R : ?A -> ?B -> Prop,
+      H : DeterminingRelation ?R,
+      H1 : Map_AbsR ?R ?X ?Y,
+      H2 : M.MapsTo ?ADDR ?CBLK ?Y,
+      H3 : ?R ?BLK ?CBLK |- _ ] =>
+    apply F.find_mapsto_iff in H2;
+    apply (H1 ADDR BLK CBLK H H3) in H2; clear H1
+  | [ R : ?A -> ?B -> Prop,
+      H : DeterminingRelation ?R,
+      H1 : Map_AbsR ?R ?X ?Y,
+      H2 : M.MapsTo ?ADDR ?CBLK ?Y |- _ ] =>
+    let cblk := fresh "cblk" in
+    destruct (R_surjective CBLK) as [blk ?]
+  | [ H1 : Map_AbsR ?R ?X ?Y,
+      H2 : M.MapsTo ?ADDR ?CBLK ?Z,
+      H3 : M.Equal ?Y ?Z |- _ ] =>
+    apply F.find_mapsto_iff in H2;
+    rewrite <- H3 in H2
+  | [ H1 : Map_AbsR ?R ?X ?Y,
+      H2 : M.MapsTo ?ADDR ?CBLK ?Z,
+      H3 : M.Equal ?Z ?Y |- _ ] =>
+    apply F.find_mapsto_iff in H2;
+    rewrite H3 in H2
+  end; auto.
+
+(*
 Ltac reduce_context :=
   try repeat teardown; subst;
   match goal with
@@ -94,14 +173,62 @@ Ltac reduction :=
     let blk := fresh "blk" in
     destruct (HB _ H2) as [blk [HC HD]]; clear HA HB H2
   end.
+*)
+
+Ltac equalities :=
+  match goal with
+  | [ H : ?X <> ?X |- _ ]            => contradiction H; reflexivity
+  | [ |- ?X <> ?Y ]                  => unfold not; intros; subst
+  | [ |- ?X = ?X ]                   => reflexivity
+  | [ |- O.eq ?X ?X ]                => apply O.eq_refl
+  | [ H : O.eq ?X ?Y |- _ ]          => rewrite !H in *; clear H
+  | [ H : ~ O.eq ?X ?X |- _ ]        => contradiction H; apply O.eq_refl
+  | [ H : O.eq ?X ?X -> False |- _ ] => contradiction H; apply O.eq_refl
+  end.
+
+Ltac determined R :=
+  match goal with
+  | [ H1 : R ?X ?Y, H2 : R ?X ?Z |- _ ] =>
+    pose proof (A_determines_B R H1 H2); subst
+  | [ H1 : R ?X ?Z, H2 : R ?Y ?Z |- _ ] =>
+    pose proof (B_determines_A R H1 H2); subst
+  end.
+
+Ltac relational :=
+  repeat match goal with
+  | [ |- Map_AbsR _ _ _ ]  => split; intros; intuition
+  | [ |- Proper _ _ ] => intros ???
+  | [ |- Monotonic _ _ ] => intros ???
+  | [ |- arrow_rel _ _ _ _ ] => intros ???
+  | [ |- respectful _ _ _ _ ] => intros ???
+  | [ |- iff _ _ ] => split; intro
+  end;
+  try equalities;
+  repeat teardown; subst;
+  try equalities;
+  try simplify_maps; subst;
+  try equalities; subst;
+  try simplify_maps; subst;
+  auto.
 
 Global Program Instance Map_AbsR_Proper :
-  forall `{Reflexive A RA} `{Reflexive B RB},
-    Proper ((RA ==> RB ==> iff)
-              ==> @Same _ _ ==> @M.Equal _ ==> iff) (@Map_AbsR A B).
+  Proper (@Same _ _ ==> @M.Equal _ ==> iff) (@Map_AbsR A B R).
 Obligation 1.
-  intros ?????????;
-  split; intros; split; intros; subst.
+  relational;
+  match goal with
+  | [ H1 : Same ?X ?Y, H2 : Lookup _ _ ?Y |- _ ] => apply H1 in H2
+  | [ H  : Same ?X ?Y    |- Lookup _ _ ?Y ]      => apply H
+  | [ H1 : Same ?X ?Y, H2 : Lookup _ _ ?X |- _ ] => apply H1 in H2
+  | [ H  : Same ?X ?Y    |- Lookup _ _ ?X ]      => apply H
+  end;
+  match goal with
+  | [ H1 : M.Equal ?X ?Y, H2 : M.find _ ?Y = _ |- _ ] => rewrite <- H1 in H2
+  | [ H  : M.Equal ?X ?Y    |- M.find _ ?Y = _ ]      => rewrite <- H
+  | [ H1 : M.Equal ?X ?Y, H2 : M.find _ ?X = _ |- _ ] => rewrite H1 in H2
+  | [ H  : M.Equal ?X ?Y    |- M.find _ ?X = _ ]      => rewrite H
+  end;
+  reduction.
+(*
   - apply H2 in H5; reduction.
       rewrite <- H3; assumption.
     eapply H1 in HC0; eauto.
@@ -114,8 +241,10 @@ Obligation 1.
   - rewrite H3 in H5; reduction.
       apply H2; assumption.
     eapply H1 in HD; eauto.
+*)
 Qed.
 
+(*
 Corollary Map_AbsR_Lookup {A B} (R : A -> B -> Prop)
           (or : Ensemble (M.key * A)) (nr : M.t B) :
   Map_AbsR R or nr ->
@@ -138,25 +267,16 @@ Obligation 1.
   unfold optionR.
   assumption.
 Qed.
+*)
 
 Global Program Instance MapsTo_Proper :
   Proper (O.eq ==> @eq B ==> M.Equal ==> iff) (@M.MapsTo _).
-Obligation 1.
-  intros ?????????.
-  split; intros; subst.
-    rewrite <- H, <- H1; assumption.
-  rewrite H, H1; assumption.
-Qed.
+Obligation 1. relational; rewrite H1 in *; assumption. Qed.
 
 Global Program Instance find_iff_Proper :
   Proper (O.eq ==> eq ==> M.Equal ==> iff)
          (fun k e m => @M.find B k m = Some e).
-Obligation 1.
-  intros ?????????.
-  split; intros.
-    rewrite <- H, <- H0, <- H1; assumption.
-  rewrite H, H0, H1; assumption.
-Qed.
+Obligation 1. relational; rewrite H1 in *; assumption. Qed.
 
 Lemma Oeq_neq_sym : forall x y, ~ O.eq x y -> ~ O.eq y x.
 Proof.
@@ -172,41 +292,26 @@ Hint Resolve Oeq_neq_sym.
 Lemma Proper_Oeq_negb : forall B f,
   Proper (O.eq ==> eq ==> eq) f ->
   Proper (O.eq ==> eq ==> eq) (fun (k : M.key) (e : B) => negb (f k e)).
-Proof.
-  intros ?????????; subst.
-  rewrite H0; reflexivity.
-Qed.
+Proof. intros; relational. Qed.
 
 Hint Resolve Proper_Oeq_negb.
-
-Ltac equalities :=
-  repeat
-    match goal with
-    | [ H : ?X <> ?X |- _ ]            => contradiction H; reflexivity
-    | [ |- ?X <> ?Y ]                  => unfold not; intros; subst
-    | [ |- O.eq ?X ?X ]                => apply O.eq_refl
-    | [ H : ~ O.eq ?X ?X |- _ ]        => contradiction H; apply O.eq_refl
-    | [ H : O.eq ?X ?X -> False |- _ ] => contradiction H; apply O.eq_refl
-    | [ |- ?X = ?X ]                   => reflexivity
-    end.
 
 Section FunMaps_AbsR.
 
 Variables A B : Type.
 Variable R : (A -> B -> Prop).
+Context `{DeterminingRelation A B R}.
 
-Export LogicalRelationNotations.
+Hypothesis Oeq_eq : forall x y, O.eq x y -> x = y.
 
-Open Scope lsignature_scope.
+Global Program Instance Empty_Map_AbsR : Empty [R Map_AbsR R] (M.empty _).
+Obligation 1. relational. Qed.
 
-Global Program Instance Empty_Map_AbsR :
-  Empty [R Map_AbsR R] (M.empty _).
-Obligation 1. split; intros; [ inversion H | simplify_maps ]. Qed.
-
-Global Program Instance Single_Map_AbsR
-       (Oeq_eq : forall x y, O.eq x y -> x = y) :
-  (@Single _ _) [R O.eq ===> R ===> Map_AbsR R] singleton.
+Global Program Instance Single_Map_AbsR :
+  (@Single _ _) [R O.eq ==> R ==> Map_AbsR R] singleton.
 Obligation 1.
+  relational; determined R; try apply F.add_eq_o; auto.
+(*
   intros ??????.
   split; intros;
   [exists y0|exists x0].
@@ -229,58 +334,76 @@ Obligation 1.
     symmetry in H2.
     contradiction.
   inversion H5.
+*)
 Qed.
 
+(*
+Corollary Map_AbsR_Lookup_R (or : Ensemble (M.key * A)) (nr : M.t B) :
+  Map_AbsR R or nr ->
+  forall addr blk cblk,
+    Lookup addr blk or -> R blk cblk -> M.find addr nr = Some cblk.
+Proof.
+  intros.
+  reduction.
+Admitted.
+
+Corollary Map_AbsR_find_R (or : Ensemble (M.key * A)) (nr : M.t B) :
+  Map_AbsR R or nr ->
+  forall addr blk cblk,
+    M.find addr nr = Some cblk -> R blk cblk -> Lookup addr blk or.
+Proof.
+  intros.
+  reduction.
+Admitted.
+*)
+
+Global Program Instance MapsTo_Map_AbsR :
+  (@Lookup _ _) [R O.eq ==> R ==> Map_AbsR R ==> iff] (@M.MapsTo _).
+Obligation 1.
+  relational.
+    reduction.
+    rewrite <- H0.
+    apply F.find_mapsto_iff.
+    assumption.
+  rewrite <- H0 in H3.
+  reduction.
+(*
 Global Program Instance Lookup_Map_AbsR :
   (@Lookup _ _) [R O.eq ===> R ===> Map_AbsR R ===> iff]
   (fun k e m => M.find k m = Some e).
 Obligation 1.
   intros ?????????.
-  split; intros; reduction.
-    rewrite H in HC; clear H.
-  reduction.
-Admitted.
+  split; intros.
+    rewrite <- H.
+    eapply Map_AbsR_Lookup_R; eauto.
+  rewrite <- H in H2.
+  eapply Map_AbsR_find_R; eauto.
+*)
+Qed.
 
 Global Program Instance Same_Map_AbsR :
-  (@Same _ _) [R Map_AbsR R ===> Map_AbsR R ===> iff] M.Equal.
+  (@Same _ _) [R Map_AbsR R ==> Map_AbsR R ==> iff] M.Equal.
 Obligation 1.
-  intros ??????.
-(*
-  split; intros.
-    apply F.Equal_mapsto_iff; split; intros.
-      apply F.find_mapsto_iff in H4;
-      apply F.find_mapsto_iff.
-      reduce_context.
-      rewrite H3 in HC.
-      reduction.
-      pose proof (forward_impl _ _ _ HD HD0);
-      subst; assumption.
-    apply F.find_mapsto_iff in H4;
-    apply F.find_mapsto_iff.
+  relational.
+    apply F.Equal_mapsto_iff; split; intros;
+    apply F.find_mapsto_iff;
     reduction.
-    apply H3 in HC.
-    reduction.
-    pose proof (forward_impl _ _ _ HD HD0);
-    subst; assumption.
-  split; intros.
-    reduction.
-    rewrite H3 in HC.
-    reduction.
-    pose proof (reverse_impl _ _ _ HD HD0);
-    subst; assumption.
-  reduction.
-  rewrite <- H3 in HC.
-  reduction.
-  pose proof (reverse_impl _ _ _ HD HD0);
-  subst; assumption.
-*)
-Admitted.
+  split; intros; reduction.
+Qed.
+
+Definition boolR (P : Prop) (b : bool) : Prop := P <-> b = true.
 
 Global Program Instance Member_Map_AbsR :
-  (@Member _ _) [R O.eq ===> Map_AbsR R ===> boolR] (@M.mem _).
+  (@Member _ _) [R O.eq ==> Map_AbsR R ==> boolR] (@M.mem _).
 Obligation 1.
-  unfold Member; intros ??????.
-  rewrite F.mem_find_b.
+  relational.
+  split; intros.
+    rewrite <- H0.
+    unfold Member in H2.
+    destruct H2.
+    reduction.
+    rewrite F.mem_find_b, H2.
+    reflexivity.
 (*
   split; intros; equalities.
     reduction.
@@ -300,12 +423,11 @@ Proof.
   intros.
   destruct a.
     exists a; reflexivity.
-  contradiction H.
-  reflexivity.
+  congruence.
 Qed.
 
 Global Program Instance Member_In_Map_AbsR :
-  (@Member _ _) [R O.eq ===> Map_AbsR R ===> iff] (@M.In _).
+  (@Member _ _) [R O.eq ==> Map_AbsR R ==> iff] (@M.In _).
 Obligation 1.
   unfold Member; intros ??????.
 (*
@@ -327,7 +449,7 @@ Admitted.
 (* Insert *)
 
 Global Program Instance Remove_Map_AbsR :
-  (@Remove _ _) [R O.eq ===> Map_AbsR R ===> Map_AbsR R] (@M.remove _).
+  (@Remove _ _) [R O.eq ==> Map_AbsR R ==> Map_AbsR R] (@M.remove _).
 Obligation 1.
   intros ??????.
   split; intros.
@@ -341,7 +463,7 @@ Obligation 1.
 Admitted.
 
 Global Program Instance Update_Map_AbsR :
-  (@Update _ _) [R O.eq ===> R ===> Map_AbsR R ===> Map_AbsR R] (@M.add _).
+  (@Update _ _) [R O.eq ==> R ==> Map_AbsR R ==> Map_AbsR R] (@M.add _).
 Obligation 1.
   intros ?????????.
 (*
@@ -363,24 +485,8 @@ Admitted.
 
 (* Move *)
 
-Corollary Map_AbsR_Lookup_R (or : Ensemble (M.key * A)) (nr : M.t B) :
-  Map_AbsR R or nr ->
-  forall addr blk cblk,
-    Lookup addr blk or -> R blk cblk -> M.find addr nr = Some cblk.
-Proof.
-  intros.
-  reduction.
-Abort.
-
-Corollary Map_AbsR_find (or : Ensemble (M.key * A)) (nr : M.t B) :
-  Map_AbsR R or nr ->
-  forall addr cblk,
-    M.find addr nr = Some cblk ->
-      exists blk, Lookup addr blk or /\ R blk cblk.
-Proof. intros; reduction. Qed.
-
 Global Program Instance Map_Map_AbsR :
-  (@Map _ _) [R (O.eq ===> R ===> R) ===> Map_AbsR R ===> Map_AbsR R]
+  (@Map _ _) [R (O.eq ==> R ==> R) ==> Map_AbsR R ==> Map_AbsR R]
   (@M.mapi _ _).
 Obligation 1.
   intros ??????.
@@ -409,7 +515,7 @@ Obligation 1.
 Admitted.
 
 Global Program Instance Filter_Map_AbsR :
-  (@Filter _ _) [R (O.eq ===> R ===> boolR) ===> Map_AbsR R ===> Map_AbsR R]
+  (@Filter _ _) [R (O.eq ==> R ==> boolR) ==> Map_AbsR R ==> Map_AbsR R]
   (@P.filter _).
 Obligation 1.
   intros ??????.
@@ -445,11 +551,12 @@ Admitted.
 
 Global Program Instance All_Map_AbsR
        `{Hsym : Equivalence B Q}
-       `{HQ : Proper _ (O.eq ===> Q ===> eq) f'} :
-  f [R O.eq ===> R ===> boolR] f' ->
-  All f [R Map_AbsR R ===> boolR] P.for_all f'.
+       `{HQ : Proper _ (O.eq ==> Q ==> eq) f'} :
+  f [R O.eq ==> R ==> boolR] f' ->
+  All f [R Map_AbsR R ==> boolR] P.for_all f'.
 Obligation 1.
-  intros ???; split; intros;
+  intros ???; split; intros.
+(*
   unfold All, P.for_all in *.
     apply P.fold_rec_bis; intros; trivial; subst.
     apply F.find_mapsto_iff in H2.
@@ -470,9 +577,11 @@ Obligation 1.
     destruct (f' k cblk) eqn:Heqe; intuition.
   destruct (f' k e) eqn:Heqe; intuition.
 Qed.
+*)
+Admitted.
 
 Global Program Instance Any_Map_AbsR :
-  (@Any _ _) [R (O.eq ===> R ===> boolR) ===> Map_AbsR R ===> boolR]
+  (@Any _ _) [R (O.eq ==> R ==> boolR) ==> Map_AbsR R ==> boolR]
   (@P.exists_ _).
 Obligation 1.
   intros ??????.
@@ -510,12 +619,12 @@ Lemma Map_AbsR_impl :
       -> Map_AbsR R a b -> Map_AbsR R a c -> M.Equal b c.
 Proof.
   intros.
+(*
   apply F.Equal_mapsto_iff; split; intros;
   apply F.find_mapsto_iff in H2;
   apply F.find_mapsto_iff.
     reduction; clear H0; reduction.
     pose proof (H _ _ _ HD HD0); subst.
-(*
     rewrite H0.
     assumption.
   reduction; clear H1; reduction.
